books/misc/check-acl2-exports.lisp
@@ -200,19 +200,6 @@
 
 ; Symbols below should probably be added to *acl2-exports*.
 
-    ADD-SUFFIX
-    ADD-SUFFIX-TO-FN
-    COMMENT
-    REWRITE-EQUIV
-    STANDARD-CHAR-P+
-    SUBSEQUENCEP
-
-; NOTE: DEFMACRO-UNTOUCHABLE can probably be removed from special treatment in
-; books/projects/apply-model/portcullis.lisp
-; and
-; books/projects/apply-model-2/portcullis.lisp
-; after it is added to *acl2-exports*.
-    DEFMACRO-UNTOUCHABLE UNTOUCHABLE-MARKER
   ))
 
 (defconst *special-ops*
