books/projects/apply/copy-nat-tree.lisp
@@ -1,0 +1,295 @@
+; Copyright (C) 2020, Regents of the University of Texas
+; Written by Matt Kaufmann and J Moore
+; License: A 3-clause BSD license.  See the LICENSE file distributed with ACL2.
+
+; Many thanks to ForrestHunt, Inc. for supporting the preponderance of this
+; work, and for permission to include it here.
+
+; A Brief Tutorial on Loop$ Recursion Induction
+; J Strother Moore
+; March, 2020
+
+; Abstract: This book contains inductive theorems about a rather silly but
+; instructive loop$-recursive function.  We introduce a data structure called a
+; ``nat tree,'' an example of which is (NATS (NATS 1 2 3) 4 (NATS 5 6)), and a
+; function that copies such a tree, and we prove that the copy function indeed
+; copies.  We illustrate some of the principles mentioned in :doc
+; loop$-recursion-induction.  We also relate the loop$-recursive copy function
+; to its mutually-recursive version and to a flagged function capturing that
+; mutual recursion.
+
+; Since ACL2 does not automatically compute appropriate induction schemes for
+; loop$-recursive functions, we have to provide an explicit :induction hint.
+; We regard this burden (which we would normally consider a burden) as salutary
+; here because it clearly shows what has to be done for this particular
+; loop$-recursive function.  This should enable the reader to either use this
+; same methodology in his or her own proofs about loop$-recursive functions or
+; to automate the methodology with some helpful book.  However, we are working
+; on such a book ourselves and this file illustrates the direction of our
+; thinking.
+
+; All theorems proved in this book have rule-classes nil so we can be confident
+; that proofs are not dependent on proving one theorem before another.
+
+(in-package "ACL2")
+
+(include-book "projects/apply/top" :dir :system)
+(include-book "misc/eval" :dir :system)
+
+; -----------------------------------------------------------------
+; Definitions
+
+; Here is the definition of nat-treep, two examples illustrating the predicate,
+; and the function that copies nat trees.  Both functions use loop$ recursion.
+; The copy function, copy-nat-tree, is unnecessarily complicated because it
+; copies the natural numbers in it.  That is, it reconstructs each natural by
+; adding 1 to the result of copying the non-0 predecessor natural.  We do this
+; to illustrate recursion and induction both inside and outside the loop$.
+
+(defun$ nat-treep (x)
+  (declare (xargs :loop$-recursion t
+                  :measure (acl2-count x)))
+  (cond
+   ((atom x) (natp x))
+   (t (and (true-listp x)
+           (eq (car x) 'NATS)
+           (loop$ for e in (cdr x) always (nat-treep e))))))
+
+(defthm examples-of-nat-treep
+  (implies
+   (warrant nat-treep)
+   (and (equal (nat-treep '(nats
+                            (nats 1 2 3)
+                            4
+                            (nats 5 (nats 6 7 8) 9))) t)
+        (equal (nat-treep '(nats (nats 1 2 3) bad)) nil)))
+  :rule-classes nil)
+
+(defun$ copy-nat-tree (x)
+  (declare (xargs :loop$-recursion t
+                  :measure (acl2-count x)))
+  (cond
+   ((atom x)
+    (if (natp x)
+        (if (equal x 0)
+            0
+            (+ 1 (copy-nat-tree (- x 1))))
+        x))
+   (t (cons 'nats
+            (loop$ for e in (cdr x) collect (copy-nat-tree e))))))
+
+; -----------------------------------------------------------------
+; Failures Illustrating General Principles and the Induction Hint
+
+; We now illustrate the general principles mentioned in :doc
+; loop$-recursion-induction.
+
+; The following will fail for many reasons.  But the reason we want to
+; highlight is the absence of the warrants for nat-treep and copy-nat-tree!
+
+(must-fail
+ (defthm failure-0 ; no warrants!
+   (implies (nat-treep x)
+            (equal (copy-nat-tree x) x))))
+
+; We now provide the necessary warrants, but loop$-recursive functions do not
+; automatically suggest induction schemes, so this will fail.
+
+(must-fail
+ (defthm failure-1 ; no induction is suggested by loop$-recursion
+   (implies (and (warrant nat-treep copy-nat-tree)
+                 (nat-treep x))
+            (equal (copy-nat-tree x) x))))
+
+; An induction scheme appropriate for copy-nat-tree contains a ``(- x 1)''
+; induction hyp for naturals, and a car/cdr induction hyp for conses.  The
+; car/cdr induction hyp is necessary because as
+
+; (loop$ for e in x collect (copy-nat-tree e))
+
+; expands it introduces a recursive call of copy-nat-tree on (car x) and
+; ``recursive call of the loop$'' on (cdr x).
+
+(defun induction-hint (x)
+  (cond ((atom x)
+         (if (natp x)
+             (if (equal x 0)
+                 'base
+                 (induction-hint (- x 1)))
+             'base))
+        (t
+         (cons (induction-hint (car x))
+               (induction-hint (cdr x))))))
+
+; So now we offer the induction hint to the previously failing proof attempt.
+; It still fails because the formula to be proved does not tell us,
+; inductively, what (loop$ ... collect (copy-nat-tree ...)) does.
+
+(must-fail
+ (defthm failure-2 ; insufficiently strong
+   (implies (and (warrant nat-treep copy-nat-tree)
+                 (nat-treep x))
+            (equal (copy-nat-tree x) x))
+   :hints (("Goal" :induct (induction-hint x)))))
+
+; We attempt to fix that by conjoining another conjecture, this one about the
+; the loop$ statement inside the definition of copy-nat-tree.  One positive
+; contribution of this example is that it first illustrates the use of an
+; loop$/always to require that every element of (cdr x) is a nat-treep.
+
+; (loop$ for e in (cdr x) always (nat-treep e))
+
+; Generally speaking, when stating a theorem about the behavior of a loop$
+; in a loop$-recursive function you have to constrain the target appropriately
+; for the function to behave as specified.  Put another way, as we think about
+; the ``loop$ version'' of (implies (nat-treep x) (equal (copy-nat-tree x) x))
+; we need to think about the loop$ both the hypthesis and the conclusion, i.e.,
+; in nat-treep and in copy-nat-tree.
+
+; Despite this thinking, the following proof attempt fails too.  We need a
+; GENERAL statement about what the loop$ does on an arbitrary target, not just
+; on (cdr x)!
+
+(must-fail
+ (defthm failure-3 ; insufficiently strong
+   (implies (warrant nat-treep copy-nat-tree)
+            (and (implies (nat-treep x) (equal (copy-nat-tree x) x))
+                 (implies (and (true-listp x)
+                               (loop$ for e in (cdr x) always (nat-treep e)))
+                          (equal (loop$ for e in (cdr x) collect (copy-nat-tree e))
+                                 (cdr x)))))
+   :hints (("Goal" :induct (induction-hint x)))
+   :rule-classes nil))
+
+; -----------------------------------------------------------------
+; A Provable Form of the Desired Theorem
+
+; Finally, this conjunction succeeds.  It is a conjunction of our original
+; conjecture together with its loop$ version, it comes with the warrants we
+; need, the loop$ versions are phrased about a variable target, x, not just the
+; target used in the main function, and we provide an induction hint that
+; catches both (- x 1) recursion and car/cdr recursion.
+
+(defthm finally-success!
+  (implies (warrant nat-treep copy-nat-tree)
+           (and (implies (nat-treep x) (equal (copy-nat-tree x) x))
+                (implies (and (true-listp x)
+                              (loop$ for e in x always (nat-treep e)))
+                         (equal (loop$ for e in x collect (copy-nat-tree e))
+                                x))))
+  :hints (("Goal" :induct (induction-hint x)))
+  :rule-classes nil)
+
+; -----------------------------------------------------------------
+; Comparing Loop$-Recursion to the Corresponding Mutually-Recursive Definition
+
+; Next we turn to comparing the loop$-recursive function copy-nat-tree to its
+; mutual-recursion version.
+
+(mutual-recursion
+ (defun mr-copy-nat-tree (x)
+   (cond
+    ((atom x)
+     (if (natp x)
+         (if (equal x 0)
+             0
+             (+ 1 (mr-copy-nat-tree (- x 1))))
+         x))
+    (t (cons 'nats
+             (mr-copy-nat-tree-list (cdr x))))))
+
+ (defun mr-copy-nat-tree-list (x)
+   (cond
+    ((endp x) nil)
+    (t (cons (mr-copy-nat-tree (car x))
+             (mr-copy-nat-tree-list (cdr x)))))))
+
+; The following proof may come as a surprise to some ACL2 users.  It shows that
+; the induction hint that is appropriate for copy-nat-tree -- an induction that
+; uses both (- x 1) recursion and car/cdr recursion -- can be used successfully
+; on a conjunction of theorems about a mutually recursive function.
+
+(defthm mr-copy-nat-tree-copies
+  (implies (warrant nat-treep)
+           (and (implies (nat-treep x)
+                         (equal (mr-copy-nat-tree x) x))
+                (implies (and (true-listp x)
+                              (loop$ for e in x always (nat-treep e)))
+                         (equal (mr-copy-nat-tree-list x) x))))
+  :hints (("Goal" :induct (induction-hint x)))
+  :rule-classes nil)
+
+; Note also that the theorem above uses the loop$-recursive function nat-treep
+; to constrain the input to the mutually recursive functions.  Thus, we need
+; the warrant for nat-treep.
+
+; In a similiar vein, we can prove that the loop$-recursive function is
+; equivalent to its mutually recursive counterpart.
+
+(defthm copy-nat-tree-is-mr-copy-nat-tree
+  (implies (warrant nat-treep copy-nat-tree)
+           (and (implies (nat-treep x)
+                         (equal (copy-nat-tree x)
+                                (mr-copy-nat-tree x)))
+                (implies (and (true-listp x)
+                              (loop$ for e in x always (nat-treep e)))
+                         (equal (loop$ for e in x collect (copy-nat-tree e))
+                                (mr-copy-nat-tree-list x)))))
+  :hints (("Goal" :induct (induction-hint x)))
+  :rule-classes nil)
+
+; -----------------------------------------------------------------
+; Eliminating Loop$-Recursion in Favor of Flagged Mutual Recursion
+
+; Finally, another way to approach proofs about loop$-recursive functions is to
+; introduce the ``flagged mutually recursive'' version and prove equivalence.
+; We hope this approach isn't used regularly because it requires defining yet
+; another function and the beauty of loop$ recursion is that it avoids defining
+; helper functions.  However, as a last resort, you can reduce the
+; loop$-recursive function to a flagged mutually recursive function and then
+; use conventional methods to prove properties.
+
+; In the following flagged version, flg=t means x is treated as a nat-treep and
+; flg=nil means it is treated as a list of nat-treeps.
+
+(defun flagged-mr-copy-nat-tree (flg x)
+  (if flg
+      (cond
+       ((atom x)
+        (if (natp x)
+            (if (equal x 0)
+                0
+                (+ 1 (flagged-mr-copy-nat-tree t (- x 1))))
+            x))
+       (t (cons 'nats
+                (flagged-mr-copy-nat-tree nil (cdr x)))))
+      (cond
+       ((endp x) nil)
+       (t (cons (flagged-mr-copy-nat-tree t (car x))
+                (flagged-mr-copy-nat-tree nil (cdr x)))))))
+
+; Then we can prove that the flagged function is either copy-nat-tree or its
+; loop$ counterpart, depending on the flag.  No induction hint is necessary
+; because the term (flagged-mr-copy-nat-tree flg x) suggests the right
+; induction.  We still need the warrant for copy-nat-tree.
+
+(defthm flagged-equivalence
+  (implies (warrant copy-nat-tree)
+           (equal (flagged-mr-copy-nat-tree flg x)
+                  (if flg
+                      (copy-nat-tree x)
+                      (loop$ for e in x collect (copy-nat-tree e)))))
+  :rule-classes nil)
+
+; The following trivial corollary, if proved as a :rewrite rule, will
+; eliminate the loop$ recursion in favor of flagged mutual recursion.
+
+(defthm eliminate-copy-nat-tree
+  (implies (warrant copy-nat-tree)
+           (and (equal (copy-nat-tree x) (flagged-mr-copy-nat-tree t x))
+                (equal (loop$ for e in x collect (copy-nat-tree e))
+                       (flagged-mr-copy-nat-tree nil x))))
+  :hints (("Goal" :use ((:instance flagged-equivalence (flg t))
+                        (:instance flagged-equivalence (flg nil)))))
+  :rule-classes nil)
+
