books/std/util/maybe-defthm.lisp
@@ -93,8 +93,7 @@
 ; argument to have had remove-guard-holders applied.
 
                                                 (acl2::remove-guard-holders
-                                                 concl
-                                                 wrld)
+                                                 concl)
                                                 ens wrld))
          ((when msg)
           ;; Not okay!  Don't submit the theorem.
@@ -122,3 +121,38 @@
       (if (is-theorem-p name (w state))
           (value `(in-theory (disable ,name)))
         (value `(value-triple :invisible))))))
+
+(local
+ (progn
+
+   ;; Some basic tests
+
+   (include-book "misc/assert" :dir :system)
+
+   (maybe-defthm-as-rewrite foo (equal (car (cons x y)) x))
+   (maybe-defthm-as-rewrite bar (equal (not 'nil) 't))
+   (maybe-defthm-as-rewrite baz (equal (stringp 'nil) 'nil))
+
+   (assert! (is-theorem-p 'foo (w state)))
+   (assert! (not (is-theorem-p 'bar (w state))))
+   (assert! (not (is-theorem-p 'baz (w state))))
+
+   (assert! (let ((acl2::ens (acl2::ens state))) (active-runep '(:rewrite foo))))
+   (assert! (let ((acl2::ens (acl2::ens state))) (not (active-runep '(:rewrite bar)))))
+
+   (enable-if-theorem foo)
+
+   (assert! (let ((acl2::ens (acl2::ens state)))
+              (active-runep '(:rewrite foo))))
+
+   (disable-if-theorem foo)
+
+   (assert! (let ((acl2::ens (acl2::ens state)))
+              (not (active-runep '(:rewrite foo)))))
+
+   (enable-if-theorem foo)
+
+   (assert! (let ((acl2::ens (acl2::ens state)))
+              (active-runep '(:rewrite foo))))
+
+   ))
