defthm.lisp
@@ -1666,7 +1666,10 @@
 ; is a ttree that justifies the storage of all the :REWRITE rules.
 
   (chk-acceptable-rewrite-rule1 name match-free loop-stopper
-                                (unprettyify (remove-guard-holders term wrld))
+                                (unprettyify
+                                 (possibly-clean-up-dirty-lambda-objects
+                                  (remove-guard-holders term)
+                                  wrld))
                                 ctx ens wrld state))
 
 ; So now we work on actually generating and adding the rules.
@@ -1772,7 +1775,10 @@
 ; convention.  "Consistency is the hobgoblin of small minds."  Emerson?
 
   (add-rewrite-rule1 rune nume
-                     (unprettyify (remove-guard-holders term wrld))
+                     (unprettyify
+                      (possibly-clean-up-dirty-lambda-objects
+                       (remove-guard-holders term)
+                       wrld))
                      loop-stopper-lst backchain-limit-lst match-free ens wrld))
 
 ;---------------------------------------------------------------------------
@@ -2253,7 +2259,10 @@
 ; messages without causing an error.
 
   (chk-acceptable-linear-rule1 name match-free trigger-terms
-                               (unprettyify (remove-guard-holders term wrld))
+                               (unprettyify
+                                (possibly-clean-up-dirty-lambda-objects
+                                 (remove-guard-holders term)
+                                 wrld))
                                ctx ens wrld state))
 
 ; And now, to adding :LINEAR rules...
@@ -2300,7 +2309,9 @@
 
 (defun add-linear-rule2 (rune nume trigger-terms hyps concl
                               backchain-limit-lst match-free ens wrld state)
-  (let* ((concl (remove-guard-holders concl wrld))
+  (let* ((concl (possibly-clean-up-dirty-lambda-objects
+                 (remove-guard-holders concl)
+                 wrld))
          (xconcl (expand-inequality-fncall concl))
          (lst (external-linearize xconcl ens wrld state))
          (hyps (preprocess-hyps hyps wrld))
@@ -2365,7 +2376,10 @@
 ;                (recur-over-break-cons cdr)))))
 
   (add-linear-rule1 rune nume trigger-terms
-                    (unprettyify (remove-guard-holders term wrld))
+                    (unprettyify
+                     (possibly-clean-up-dirty-lambda-objects
+                      (remove-guard-holders term)
+                      wrld))
                     backchain-limit-lst match-free ens wrld state))
 
 ;---------------------------------------------------------------------------
@@ -3218,7 +3232,7 @@
 ; might have.  But we decided to stick with the ``just do what the user said''
 ; approach.
 
-;   (let ((term (remove-lambdas (remove-guard-holders term wrld))))
+;   (let ((term (remove-lambdas (remove-guard-holders term))))
 ;     (cond ((or (variablep term)
 ;                (fquotep term)
 ;                (not (eq (ffn-symb term) 'implies)))
@@ -3234,7 +3248,10 @@
 ;                                hyps)
 ;                        concls)))))
 
-  (let ((term (remove-lambdas (remove-guard-holders term wrld))))
+  (let ((term (remove-lambdas
+               (possibly-clean-up-dirty-lambda-objects
+                (remove-guard-holders term)
+                wrld))))
     (cond ((or (variablep term)
                (fquotep term)
                (not (eq (ffn-symb term) 'implies)))
@@ -3717,8 +3734,9 @@
                        cl-set0
                        (normalized-evaluator-cl-set evfn-lst wrld)))
                      (cl-set2
-                      (remove-guard-holders-lst-lst
-                       (evaluator-clauses evfn evfn-lst fn-args-lst)
+                      (possibly-clean-up-dirty-lambda-objects-lst-lst
+                       (remove-guard-holders-lst-lst
+                        (evaluator-clauses evfn evfn-lst fn-args-lst))
                        wrld)))
                 (cond
                  ((not (and (clause-set-subsumes nil cl-set1 cl-set2)
@@ -5362,7 +5380,9 @@
 ; type-set lemmas in wrld.  The ttree returned contains no 'assumption
 ; tags.
 
-  (let ((term (remove-guard-holders term wrld)))
+  (let ((term (possibly-clean-up-dirty-lambda-objects
+               (remove-guard-holders term)
+               wrld)))
     (mv-let
      (hyps concl)
      (unprettyify-tp term)
@@ -6454,7 +6474,10 @@
 ; are so intermingled that it seemed dubious to separate them into two
 ; functions.
 
-  (let ((pairs (unprettyify (remove-guard-holders term wrld)))
+  (let ((pairs (unprettyify
+                (possibly-clean-up-dirty-lambda-objects
+                 (remove-guard-holders term)
+                 wrld)))
         (hyp-msg   "~x0 is an unacceptable :CONGRUENCE rule.  The ~
                     single hypothesis of a :CONGRUENCE rule must be a ~
                     term of the form (equiv x y), where equiv has ~
@@ -7834,7 +7857,7 @@
 ; for a :definition rule with the indicated formals and body.  We guess a
 ; :controller-alist or cause an error.
 
-  (let ((t-machine (termination-machine names body nil nil
+  (let ((t-machine (termination-machine nil nil names formals body nil nil
                                         (default-ruler-extenders wrld))))
     (er-let*
      ((m (guess-measure (car names) nil formals 0 t-machine ctx wrld state)))
@@ -8494,7 +8517,10 @@
       (cond ((not (assoc-eq :TYPED-TERM seen))
              (mv-let
               (hyps concl)
-              (unprettyify-tp (remove-guard-holders corollary wrld))
+              (unprettyify-tp
+               (possibly-clean-up-dirty-lambda-objects
+                (remove-guard-holders corollary)
+                wrld))
               (declare (ignore hyps))
               (let ((pat (cond ((ffn-symb-p concl 'implies)
                                 (find-type-prescription-pat (fargn concl 2)
@@ -8770,11 +8796,17 @@
                               See :DOC linear."
                              name))
                         (t
-                         (let ((terms (remove-guard-holders-lst terms wrld)))
+                         (let ((terms
+                                (possibly-clean-up-dirty-lambda-objects-lst
+                                 (remove-guard-holders-lst terms)
+                                 wrld)))
                            (er-progn
                             (chk-legal-linear-trigger-terms
                              terms
-                             (unprettyify (remove-guard-holders corollary wrld))
+                             (unprettyify
+                              (possibly-clean-up-dirty-lambda-objects
+                               (remove-guard-holders corollary)
+                               wrld))
                              name ctx state)
                             (value terms)))))))
                     ((eq token :FORWARD-CHAINING)
@@ -8787,8 +8819,10 @@
                                    one trigger.  Your rule class, ~x0, ~
                                    specifies none.  See :DOC forward-chaining."
                                   x))
-                             (t (value (remove-guard-holders-lst terms
-                                                                 wrld))))))
+                             (t (value
+                                 (possibly-clean-up-dirty-lambda-objects-lst
+                                  (remove-guard-holders-lst terms)
+                                  wrld))))))
                     (t
                      (er soft ctx
                          ":TRIGGER-TERMS can only be specified for ~
@@ -8935,12 +8969,16 @@
                             (:type-prescription
                              (mv-let
                               (hyps concl)
-                              (unprettyify-tp (remove-guard-holders corollary
-                                                                    wrld))
+                              (unprettyify-tp
+                               (possibly-clean-up-dirty-lambda-objects
+                                (remove-guard-holders corollary)
+                                wrld))
                               (list (cons hyps concl))))
                             (otherwise
-                             (unprettyify (remove-guard-holders corollary
-                                                                wrld))))))
+                             (unprettyify
+                              (possibly-clean-up-dirty-lambda-objects
+                               (remove-guard-holders corollary)
+                               wrld))))))
                      (cond
                       ((not (member-eq token
                                        '(:REWRITE :META :LINEAR
@@ -11196,9 +11234,11 @@
 
             (let ((attached-fns
                    (attached-fns (canonical-ancestors-lst
-                                  (all-ffn-symbs (remove-guard-holders tterm
-                                                                       wrld)
-                                                 nil)
+                                  (all-ffn-symbs
+                                   (possibly-clean-up-dirty-lambda-objects
+                                    (remove-guard-holders tterm)
+                                    wrld)
+                                   nil)
                                   wrld)
                                  wrld)))
               (cond
