other-events.lisp
@@ -6354,15 +6354,12 @@
 ; (perhaps more than is necessary), we avoid removing guard holders from quoted
 ; lambdas by passing in nil as the second argument of remove-guard-holders-lst.
 
+; It might be sound to clean up dirty lambdas here, as is our convention when
+; calling remove-guard-holders, but we are playing it safe here.  If that
+; causes problems then we can think harder about whether it is sound.
+
            (remove-guard-holders-lst
-            (constraints-list infectious-fns wrld formula-lst1 nil)
-
-; It might be sound to pass in the world hereso that guard holders are removed
-; from quoted lambdas in argument positions with ilk :fn (or :fn?), but rather
-; than take a chance, we are playing it safe here.  If that causes problems
-; then we can think harder about whether it is sound to pass in the world here.
-
-            nil)))
+            (constraints-list infectious-fns wrld formula-lst1 nil))))
      (mv constraints constrained-fns subversive-fns infectious-fns fns))))
 
 (defun bogus-exported-compliants (names exports-with-sig-ancestors sig-fns
@@ -24160,7 +24157,9 @@
             (cond ((or (variablep term)
                        (fquotep term)
                        (flambdap (ffn-symb term)))
-                   (mv t (remove-guard-holders term wrld)))
+                   (mv t (possibly-clean-up-dirty-lambda-objects
+                          (remove-guard-holders term)
+                          wrld)))
                   (t (mv nil term)))
             (cond ((or (variablep term1)
                        (fquotep term1)
